---
title: "Deriving the poisson distribution from binomial"
author: "Chris Kelly"
date: '02-28-24'
categories: [Binomial, Poisson]
format:
  html:
    code-fold: true
image: '../images/fundamentals_binom_pois.png'    
---

::: {.callout-tip}
### What are we exploring?
How extending the binomial distribution to an infinite number of trials derives the poisson distribution.
:::

## Defining a binomial problem

Let's look at a metric for the number of failures of an autonomous driving system per 100,000 km driven.

We could model this using the binomial probability density, where we define each km driven as a trial, and an event being a failure occuring during a km driven:

$$
\displaylines{
\begin{align}
P(x) = & 
{n \choose x} p^x (1-p)^{n-x}
\\\\ \text{where } n & \text{ is total miles driven}
\\ \text{and } x & \text{ is number of failures}
\end{align}
}
$$

## Increasing the number of trials to infinity

What happens if we test billions of miles? This is effectively the same as asking what happens if $n \rightarrow \infty$.

Let's also define $\lambda$, the mean number of successes we expect over $n$ trials (the "rate"). This simply means that $\lambda = np$

$$
\displaylines{
\begin{align}
\lim_{n \rightarrow \infty} & 
{n \choose x} p^x (1-p)^{n-x}
\\
= \lim_{n \rightarrow \infty} & 
{n \choose x} \left( \frac{\lambda}{n} \right)^x \left( 1-\frac{\lambda}{n} \right)^{(n-x)}
& \because \lambda = np
\end{align}
}
$$

It is helpful to simplify the expression before examining what happens when $n$ tends to infinity. We can split it into four parts (i, ii, iii and iv): 

$$
\displaylines{
\begin{align}
\lim_{n \rightarrow \infty} & 
{n \choose x} \left( \frac{\lambda}{n} \right)^x \left( 1-\frac{\lambda}{n} \right)^{(n-x)}
\\
= \lim_{n \rightarrow \infty} & 
\frac{n!}{(n-x)! \times x!} \times \left( \frac{\lambda}{n} \right)^x \times \left( 1-\frac{\lambda}{n} \right)^{n} \times \left( 1-\frac{\lambda}{n} \right)^{-x} 
\\
= \lim_{n \rightarrow \infty} & 
\underbrace{
  \frac{n!}{(n-x)! \times n^x} 
}_{\text{i}}
\times 
\underbrace{
  \frac{\lambda^x}{x!}
}_{\text{ii}}
\times 
\underbrace{
  \left( 1-\frac{\lambda}{n} \right)^{n} 
}_{\text{iii}}
\times
\underbrace{
   \left( 1-\frac{\lambda}{n} \right)^{-x} 
}_{\text{iv}}
\end{align}
}
$$

We now explore what happens if we extend $n$ towards infinity for each term.

#### Term i

We can expand out the factorial to simplify it:
$$
\displaylines{
\begin{align}
\frac{n!}{(n-x)! \times (n^x)} 
& = 
\frac{
  n \times (n-1) \times (n-2) \times \ldots \times 
  (n-x+1) \times \cancel{(n-x)!}
}{
  \cancel{(n-x)!} \times (n^x)
} 
\\\\ & =
\frac{n}{n} \times
\frac{n-1}{n} \times
\frac{n-2}{n} \times
\ldots \times
\frac{n-x-2}{n} \times
\frac{n-x-1}{n}
\\\\ & =
1 \times
\left( 1 - \frac{1}{n} \right) \times
\left( 1 - \frac{2}{n} \right) \times
\ldots \times
\left( 1 - \frac{x-2}{n} \right) \times
\left( 1 - \frac{x-1}{n} \right)
\\\\ & =
\prod_{i=1}^{x-1}{\left(1-\frac{i}{n}\right)}
\end{align}
}
$$

As similarly to before $n \rightarrow \infty$, then $\frac{i}{n} \rightarrow 0$.

$$
\displaylines{
\begin{align}
\therefore
\lim_{n \rightarrow \infty}
\prod_{i=1}^{x-1}{\left(1-\frac{i}{n}\right)}
& = 1
\end{align}
}
$$

#### Term ii

$$
\displaylines{
\begin{align}
\lim_{n \rightarrow \infty}
\frac{\lambda^x}{x!}
& =
\frac{\lambda^x}{x!}
& \because
n \text{ does not blow up}
\end{align}
}
$$

#### Term iii

This is a tricky one! 

$$
\lim_{n \rightarrow \infty}{ \left[
    \left(1 - \frac{\lambda}{n} \right)^{n}
  \right]} = e^{-\lambda}
$$

*(We go through this derivation in the footnotes for if you do not know it already)*[^1]

#### Term iv

As $n \rightarrow \infty$, then $\frac{\lambda}{n} \rightarrow 0$, so:

$$
\lim_{n \rightarrow \infty}\left( 1-\frac{\lambda}{n} \right)^{-x} = (1-0)^{-x} = 1
$$

## Tying it all together

$$
\displaylines{
\begin{align}
& \lim_{n \rightarrow \infty}
\left[
  \frac{n!}{(n-x)! \times n^x}
\times 
  \frac{\lambda^x}{x!}
\times 
  \left( 1-\frac{\lambda}{n} \right)^{n} 
\times
   \left( 1-\frac{\lambda}{n} \right)^{-x}
\right]
\\ & = 
1 \times 
  \frac{\lambda^x}{x!}
\times 
  e^{-\lambda}
\times
   1
\\ & = 
\frac{\lambda^x e^{-\lambda}}{x!}
\end{align}
}
$$

Which is the poisson pdf! 

Fin.

[^1]:
  Showing $\lim_{n \rightarrow \infty}{ \left[ \left(1 + \frac{x}{n} \right)^{n} \right]} = e^x$:
$$
\displaylines{
\begin{align}
\text{Let } f(x) & = \ln{(x)} \\
\therefore f'(x) & = \frac{1}{x} \\
\text{and } f'(x) & = 
\lim_{a \rightarrow 0}{ \left[
  \frac{f(x+a) - f(x)}{(x+a) - x}
\right] } \\
& = \lim_{a \rightarrow 0}{ \left[
  \frac{\ln{(x+a)} - \ln{(x)}}{a}
\right] }  \\
& = \lim_{a \rightarrow 0}{ \left[
  \frac{1}{a}  \ln{\left(\frac{x+a}{x} \right)} 
\right] } \\
& = \lim_{a \rightarrow 0}{ \left[
  \ln{\left(1 + \frac{a}{x} \right)^{\frac{1}{a}}} 
\right] } \\
& = \lim_{b \rightarrow \infty}{ \left[
  \ln{\left(1 + \frac{1}{bx} \right)^{b}} 
\right] } 
& \text{where } b = \frac{1}{a}
\\
& = \lim_{n \rightarrow \infty}{ \left[
  \ln{\left(1 + \frac{x}{n} \right)^{n}} 
\right]^{1/x^2} } 
& \text{where } n = bx^2
\\ 
& = \frac{1}{x} 
\\
\therefore 
e^{1/x} & = \lim_{n \rightarrow \infty}{ \left[
  \left(1 + \frac{x}{n} \right)^{n}
\right]^{1/x^2} }
\\
\therefore 
e^{x} & = \lim_{n \rightarrow \infty}{ \left[
  \left(1 + \frac{x}{n} \right)^{n}
\right]}
\end{align}
}
$$
